src/ParametricWf.v
@@ -134,6 +134,16 @@ Section ValidRegs.
       inv H; constructor; auto.
     Qed.
 
+    Lemma validRegsMetaRules_app_inv:
+      forall r1 r2,
+        ValidRegsMetaRules (r1 ++ r2) ->
+        ValidRegsMetaRules r1 -> ValidRegsMetaRules r2.
+    Proof.
+      induction r1; simpl; intros; auto.
+      inv H; inv H0.
+      firstorder fail.
+    Qed.
+
     Definition ValidRegsMetaMeth md :=
       match md with
       | OneMeth d _ => forall v, ValidRegsSinAction (projT2 d type v)
@@ -157,12 +167,127 @@ Section ValidRegs.
       inv H; constructor; auto.
     Qed.
 
+    Lemma validRegsMetaMeths_app_inv:
+      forall dms1 dms2,
+        ValidRegsMetaMeths (dms1 ++ dms2) ->
+        ValidRegsMetaMeths dms1 -> ValidRegsMetaMeths dms2.
+    Proof.
+      induction dms1; simpl; intros; auto.
+      inv H; inv H0.
+      firstorder fail.
+    Qed.
   End Regs.
 
-  Fixpoint ValidRegsMetaModule (mm: MetaModule): Prop :=
-    ValidRegsMetaRules (metaRegs mm) (metaRules mm) /\
-    ValidRegsMetaMeths (metaRegs mm) (metaMeths mm).
+  Section Regs2.
+    Variable regs: list NameRec.
 
+    Inductive ValidSinRegsSinAction:
+      forall {retT}, SinActionT type retT -> Prop :=
+    | SSVRMCall:
+        forall name sig ar {retT} cont,
+          (forall t, ValidSinRegsSinAction (cont t)) ->
+          ValidSinRegsSinAction (SMCall (lretT:= retT) name sig ar cont)
+    | SSVRLet:
+        forall {argT retT} ar cont,
+          (forall t, ValidSinRegsSinAction (cont t)) ->
+          ValidSinRegsSinAction (SLet_ (lretT':= argT) (lretT:= retT) ar cont)
+    | SSVRReadReg:
+        forall {retT} reg k cont,
+          In reg regs ->
+          (forall t, ValidSinRegsSinAction (cont t)) ->
+          ValidSinRegsSinAction (SReadReg (lretT:= retT) reg k cont)
+    | SSVRWriteReg:
+        forall {writeT retT} reg e cont,
+          In reg regs ->
+          ValidSinRegsSinAction cont ->
+          ValidSinRegsSinAction (SWriteReg (k:= writeT) (lretT:= retT)
+                                           reg e cont)
+    | SSVRIfElse:
+        forall {retT1 retT2} ce (ta fa: SinActionT type retT1)
+               (cont: type retT1 -> SinActionT type retT2),
+          ValidSinRegsSinAction ta ->
+          ValidSinRegsSinAction fa ->
+          (forall t, ValidSinRegsSinAction (cont t)) ->
+          ValidSinRegsSinAction (SIfElse ce ta fa cont)
+    | SSVRAssert:
+        forall {retT} e cont,
+          ValidSinRegsSinAction cont ->
+          ValidSinRegsSinAction (SAssert_ (lretT:= retT) e cont)
+    | SSVRReturn:
+        forall {retT} (e: Expr type (SyntaxKind retT)),
+          ValidSinRegsSinAction (SReturn e).
+
+    Definition ValidSinRegsSinRule (rule: SinRule) :=
+      ValidSinRegsSinAction (ruleGen rule type).
+
+    Inductive ValidSinRegsSinRules: list SinRule -> Prop :=
+    | ValidSinRegsSinRulesNil: ValidSinRegsSinRules nil
+    | ValidSinRegsSinRulesCons:
+        forall rule rules,
+          ValidSinRegsSinRules rules ->
+          ValidSinRegsSinRule rule ->
+          ValidSinRegsSinRules (rule :: rules).
+
+    Lemma validSinRegsSinRules_app:
+      forall r1 r2,
+        ValidSinRegsSinRules r1 -> ValidSinRegsSinRules r2 ->
+        ValidSinRegsSinRules (r1 ++ r2).
+    Proof.
+      induction r1; simpl; intros; auto.
+      inv H; constructor; auto.
+    Qed.
+
+    Lemma validSinRegsSinRules_app_inv:
+      forall r1 r2,
+        ValidSinRegsSinRules (r1 ++ r2) ->
+        ValidSinRegsSinRules r1 -> ValidSinRegsSinRules r2.
+    Proof.
+      induction r1; simpl; intros; auto.
+      inv H; inv H0.
+      firstorder fail.
+    Qed.
+
+    Definition ValidSinRegsSinMeth md :=
+      forall v, ValidSinRegsSinAction (projT2 (methGen md) type v).
+
+    Inductive ValidSinRegsSinMeths: list SinMeth -> Prop :=
+    | ValidSinRegsSinMethsNil: ValidSinRegsSinMeths nil
+    | ValidSinRegsSinMethsCons:
+        forall dm dms,
+          ValidSinRegsSinMeths dms ->
+          ValidSinRegsSinMeth dm ->
+          ValidSinRegsSinMeths (dm :: dms).
+
+    Lemma validSinRegsSinMeths_app:
+      forall dms1 dms2,
+        ValidSinRegsSinMeths dms1 -> ValidSinRegsSinMeths dms2 ->
+        ValidSinRegsSinMeths (dms1 ++ dms2).
+    Proof.
+      induction dms1; simpl; intros; auto.
+      inv H; constructor; auto.
+    Qed.
+
+    Lemma validSinRegsSinMeths_app_inv:
+      forall dms1 dms2,
+        ValidSinRegsSinMeths (dms1 ++ dms2) ->
+        ValidSinRegsSinMeths dms1 -> ValidSinRegsSinMeths dms2.
+    Proof.
+      induction dms1; simpl; intros; auto.
+      inv H; inv H0.
+      firstorder fail.
+    Qed.
+  End Regs2.
+  
+  Fixpoint ValidRegsMetaModule (mm: MetaModules): Prop :=
+    match mm with
+      | MetaRegFile _ _ _ _ _ _ => ValidRegsMetaRules (metaModulesRegs mm) (metaModulesRules mm) /\
+                                   ValidRegsMetaMeths (metaModulesRegs mm) (metaModulesMeths mm)
+      | MetaMod (Build_MetaModule regs rules meths) => ValidRegsMetaRules regs rules /\ ValidRegsMetaMeths regs meths
+      | ConcatMetaMod m1 m2 => ValidRegsMetaModule m1 /\ ValidRegsMetaModule m2
+      | RepeatSinMod A strA goodStrFn GenK getConstK goodStrFn2 ls noDupLs m =>
+        ValidSinRegsSinRules (map (@regName _) (sinRegs m)) (sinRules m) /\
+        ValidSinRegsSinMeths (map (@regName _) (sinRegs m)) (sinMeths m)
+    end.
 End ValidRegs.
 
 (* NOTE: Defining "MetaModRegsWf" by Gallina definition affects proof automation by "kvr". *)
@@ -282,18 +407,110 @@ Section Facts.
       apply SubList_refl.
   Qed.
 
+  Lemma validSinRegsSinAction_validRegsAction:
+    forall regs ty A (strA: A -> string) GenK getConstK i k (a: SinActionT ty k),
+      ValidSinRegsSinAction regs a ->
+      ValidRegsAction
+        (map (fun x => addIndexToStr strA i (nameVal x)) regs)
+        (getGenAction strA getConstK i (convSinToGen true GenK a)).
+  Proof.
+    induction 1; simpl; intros; try (constructor; auto);
+    rewrite in_map_iff;
+    eexists; eauto.
+  Qed.
+  
+  Lemma validSinRegsSinRules_validRegsRules:
+    forall ty A regs rules,
+      ValidSinRegsSinRules ty (map (regName (A:=A)) regs) rules ->
+      forall (a: A) strA GenK getConstK,
+        ValidRegsRules ty
+                       (map (fun x : SinReg A => addIndexToStr strA a (nameVal (regName x))) regs)
+                       (map
+                          (fun sr : SinRule =>
+                             (addIndexToStr strA a (nameVal (ruleName sr))
+                                            :: (fun ty0 : Kind -> Type =>
+                                                  getGenAction strA getConstK a
+                                                               (convSinToGen true GenK (ruleGen sr ty0))))%struct)
+                          rules).
+  Proof.
+    induction rules; simpl; auto; intros; [constructor|].
+    inv H.
+    specialize (IHrules H2 a0 strA GenK getConstK).
+    constructor; auto.
+    clear - H3.
+    destruct a; simpl in *; unfold ValidSinRegsSinRule in *; simpl in *.
+    apply (validSinRegsSinAction_validRegsAction strA getConstK a0) in H3; simpl in *; rewrite map_map in H3; auto.
+  Qed.
+
+  Lemma validSinRegsSinMeths_validRegsDms:
+    forall ty A regs meths,
+      ValidSinRegsSinMeths ty (map (regName (A:=A)) regs) meths ->
+      forall (a: A) strA GenK getConstK,
+        ValidRegsDms
+          ty
+          (map (fun x : SinReg A => addIndexToStr strA a (nameVal (regName x))) regs)
+          (map
+             (fun sf : SinMeth =>
+                (addIndexToStr strA a (nameVal (methName sf))
+                               :: existT
+                               (fun sig : SignatureT =>
+                                  forall ty0 : Kind -> Type,
+                                    ty0 (arg sig) -> ActionT ty0 (ret sig)) 
+                               (projT1 (methGen sf))
+                               (fun (ty0 : Kind -> Type)
+                                    (argv : ty0 (arg (projT1 (methGen sf)))) =>
+                                  getGenAction strA getConstK a
+                                               (convSinToGen true GenK (projT2 (methGen sf) ty0 argv))))%struct)
+             meths).
+  Proof.
+    induction meths; simpl; auto; intros; [constructor|].
+    inv H.
+    specialize (IHmeths H2 a0 strA GenK getConstK).
+    constructor; auto.
+    clear - H3.
+    destruct a; simpl in *; unfold ValidSinRegsSinMeth in *; simpl in *.
+    intros.
+    specialize (H3 argV).
+    apply (validSinRegsSinAction_validRegsAction strA getConstK a0) in H3; simpl in *; rewrite map_map in H3; auto.
+  Qed.
+  
   Lemma validRegsMetaModule_validRegsModules:
     forall ty mm,
       ValidRegsMetaModule ty mm ->
-      ValidRegsModules ty (modFromMeta mm).
+      ValidRegsModules ty (modFromMetaModules mm).
   Proof.
-    destruct mm as [regs rules dms]; simpl; intros; dest; split.
-    - clear -H; induction rules; [constructor|]; inv H.
-      simpl; apply validRegsRules_app; auto.
-      apply validRegsMetaRule_validRegsRules; auto.
-    - clear -H0; induction dms; [constructor|]; inv H0.
-      simpl; apply validRegsDms_app; auto.
-      apply validRegsMetaMeth_validRegsDms; auto.
+    induction mm.
+    - simpl in *; intros; dest; split; simpl in *.
+      + constructor.
+      + unfold ValidRegsMetaModule in H; simpl in H.
+        dest.
+        inv H0.
+        inv H3.
+        clear H H2.
+        apply validRegsMetaMeth_validRegsDms in H4.
+        apply validRegsMetaMeth_validRegsDms in H5.
+        simpl in H4, H5.
+        repeat constructor; auto.
+    - intros.
+      unfold ValidRegsMetaModule in H.
+      destruct m as [regs rules dms]; simpl in *.
+      dest.
+      split.
+      + clear -H; induction rules; [constructor|]; inv H.
+        simpl in *; apply validRegsRules_app; auto.
+        apply validRegsMetaRule_validRegsRules; auto.
+      + clear -H0; induction dms; [constructor|]; inv H0.
+        simpl; apply validRegsDms_app; auto.
+        apply validRegsMetaMeth_validRegsDms; auto.
+    - intros; simpl in *; dest.
+      tauto.
+    - simpl; intros; dest.
+      unfold ValidRegsMetaModule in *.
+      clear - H H0.
+      induction ls; simpl; auto; [split; constructor |].
+      repeat split; unfold namesOf; rewrite ?map_map; simpl in *; auto; clear - H H0; unfold getActionFromGen, getMethFromGen; simpl.
+      + apply validSinRegsSinRules_validRegsRules; auto.
+      + apply validSinRegsSinMeths_validRegsDms; auto.
   Qed.
 
   Lemma validRegsSinAction_regs_weakening:
@@ -342,9 +559,9 @@ Section Facts.
    
   Lemma validRegsMetaModule_modular:
     forall ty mm1 mm2,
-      ValidRegsMetaModule ty mm1 ->
-      ValidRegsMetaModule ty mm2 ->
-      ValidRegsMetaModule ty (mm1 +++ mm2).
+      ValidRegsMetaModule ty (MetaMod mm1) ->
+      ValidRegsMetaModule ty (MetaMod mm2) ->
+      ValidRegsMetaModule ty (MetaMod (mm1 +++ mm2)).
   Proof.
     destruct mm1 as [regs1 rules1 dms1], mm2 as [regs2 rules2 dms2].
     simpl; intros; dest; split.
